theories/eris/total_primitive_laws.v
@@ -19,7 +19,7 @@ Lemma twp_alloc E v s :
   [[{ True }]] Alloc (Val v) @ s; E [[{ l, RET LitV (LitLoc l); l ↦ v }]].
 Proof.
   iIntros (Φ) "_ HΦ".
-  iApply twp_lift_atomic_head_step; [done|].
+  iApply twp_lift_atomic_head_step'; [done|].
   iIntros (? σ1) "[Hh Ht] !#".
   solve_red.
   iIntros "/=" (e2 σ2 Hs); inv_head_step.
@@ -39,7 +39,7 @@ Lemma twp_allocN_seq (N : nat) (z : Z) E v s:
   [[{ l, RET LitV (LitLoc l); [∗ list] i ∈ seq 0 N, (l +ₗ (i : nat)) ↦ v }]].
 Proof.
   iIntros (-> Hn Φ) "_ HΦ".
-  iApply twp_lift_atomic_head_step; [done|].
+  iApply twp_lift_atomic_head_step'; [done|].
   iIntros (? σ1) "[Hh Ht] !#".
   iSplit.
   { iPureIntro.
@@ -91,7 +91,7 @@ Lemma twp_load E l dq v s :
   [[{ l ↦{dq} v }]] Load (Val $ LitV $ LitLoc l) @ s; E [[{ RET v; l ↦{dq} v }]].
 Proof.
   iIntros (Φ) "Hl HΦ".
-  iApply twp_lift_atomic_head_step; [done|].
+  iApply twp_lift_atomic_head_step'; [done|].
   iIntros (? σ1) "[Hh Ht] !#".
   iDestruct (ghost_map_lookup with "Hh Hl") as %?.
   solve_red.
@@ -104,7 +104,7 @@ Lemma twp_store E l v' v s :
   [[{ RET LitV LitUnit; l ↦ v }]].
 Proof.
   iIntros (Φ) "Hl HΦ".
-  iApply twp_lift_atomic_head_step; [done|].
+  iApply twp_lift_atomic_head_step'; [done|].
   iIntros (? σ1) "[Hh Ht] !#".
   iDestruct (ghost_map_lookup with "Hh Hl") as %?.
   solve_red.
@@ -118,7 +118,7 @@ Lemma twp_rand (N : nat) (z : Z) E s :
   [[{ True }]] rand #z @ s; E [[{ (n : fin (S N)), RET #n; True }]].
 Proof.
   iIntros (-> Φ) "_ HΦ".
-  iApply twp_lift_atomic_head_step; [done|].
+  iApply twp_lift_atomic_head_step'; [done|].
   iIntros (? σ1) "Hσ !#".
   solve_red.
   iIntros (e2 σ2 Hs).
@@ -134,8 +134,8 @@ Lemma twp_alloc_tape N z E s :
   [[{ True }]] alloc #z @ s; E [[{ α, RET #lbl:α; α ↪ (N; []) }]].
 Proof.
   iIntros (-> Φ) "_ HΦ".
-  iApply twp_lift_atomic_head_step; [done|].
-  iIntros (? σ1) "(Hh & Ht) !# /=".
+  iApply twp_lift_atomic_head_step'; [done|].
+  iIntros (? σ1) "(Hh & (Ht & Hs)) !# /=".
   solve_red.
   iIntros (e2 σ2 Hs); inv_head_step.
   iMod (ghost_map_insert (fresh_loc σ1.(tapes)) with "Ht") as "[$ Hl]".
@@ -149,8 +149,8 @@ Lemma twp_rand_tape N α n ns z E s :
   [[{ α ↪ (N; n :: ns) }]] rand(#lbl:α) #z @ s; E [[{ RET #(LitInt n); α ↪ (N; ns) }]].
 Proof.
   iIntros (-> Φ) "Hl HΦ".
-  iApply twp_lift_atomic_head_step; [done|].
-  iIntros (? σ1) "(Hh & Ht) !#".
+  iApply twp_lift_atomic_head_step'; [done|].
+  iIntros (? σ1) "(Hh & (Ht & Hs)) !#".
   iDestruct (ghost_map_lookup with "Ht Hl") as %?.
   solve_red.
   iIntros (e2 σ2 Hs).
@@ -165,8 +165,8 @@ Lemma twp_rand_tape_empty N z α E s :
   [[{ α ↪ (N; []) }]] rand(#lbl:α) #z @ s; E [[{ (n : fin (S N)), RET #(LitInt n); α ↪ (N; []) }]].
 Proof.
   iIntros (-> Φ) "Hl HΦ".
-  iApply twp_lift_atomic_head_step; [done|].
-  iIntros (? σ1) "(Hh & Ht) !#".
+  iApply twp_lift_atomic_head_step'; [done|].
+  iIntros (? σ1) "(Hh & (Ht & Hs)) !#".
   iDestruct (ghost_map_lookup with "Ht Hl") as %?.
   solve_red.
   iIntros (e2 σ2 Hs).
@@ -181,8 +181,8 @@ Lemma twp_rand_tape_wrong_bound N M z α E ns s :
   [[{ α ↪ (M; ns) }]] rand(#lbl:α) #z @ s; E [[{ (n : fin (S N)), RET #(LitInt n); α ↪ (M; ns) }]].
 Proof.
   iIntros (-> ? Φ) "Hl HΦ".
-  iApply twp_lift_atomic_head_step; [done|].
-  iIntros (? σ1) "(Hh & Ht) !#".
+  iApply twp_lift_atomic_head_step'; [done|].
+  iIntros (? σ1) "(Hh & (Ht & Hs)) !#".
   iDestruct (ghost_map_lookup with "Ht Hl") as %?.
   solve_red.
   iIntros (e2 σ2 Hs).
